HOL_To_IMP-/Refinements/HOL_To_IMP_Minus_AT_MOST_THREE_SAT_To_THREE_SAT.thy
@@ -1,3 +1,4 @@
+\<^marker>\<open>creator "Kevin Kappelmann"\<close>
 theory HOL_To_IMP_Minus_AT_MOST_THREE_SAT_To_THREE_SAT
   imports
     HOL_To_IMP_Minus_SAT_To_AT_MOST_THREE_SAT
@@ -7,7 +8,72 @@ begin
 context HOL_To_HOL_Nat
 begin
 
-case_of_simps to_at_least_3_clause_eq : to_at_least_3_clause.simps
+definition "to_at_least_3_clause_empty1 i \<equiv>
+  let
+    R0 = RU (i, 0);
+    R1 = RU (i, 1);
+    R2 = RU (i, 2);
+    PR0 = Pos R0;
+    PR1 = Pos R1;
+    NR1 = Neg R1;
+    PR2 = Pos R2;
+    NR2 = Neg R2
+  in
+    [[PR0, PR1, PR2],
+    [PR0, PR1, NR2],
+    [PR0, NR1, PR2],
+    [PR0, NR1, NR2]]"
+
+function_compile_nat to_at_least_3_clause_empty1_def
+
+definition "to_at_least_3_clause_empty2 i \<equiv>
+  let
+    R0 = RU (i, 0);
+    R1 = RU (i, 1);
+    R2 = RU (i, 2);
+    NR0 = Neg R0;
+    PR1 = Pos R1;
+    NR1 = Neg R1;
+    PR2 = Pos R2;
+    NR2 = Neg R2
+  in
+    [[NR0, PR1, PR2],
+    [NR0, PR1, NR2],
+    [NR0, NR1, PR2],
+    [NR0, NR1, NR2]]"
+
+function_compile_nat to_at_least_3_clause_empty2_def
+
+definition "to_at_least_3_clause_single i x \<equiv>
+  let
+    R0 = RU (i, 0);
+    R1 = RU (i, 1);
+    PR0 = Pos R0;
+    NR0 = Neg R0;
+    PR1 = Pos R1;
+    NR1 = Neg R1
+  in
+    [[x,PR0, PR1],
+    [x, PR0, NR1],
+    [x, NR0, PR1],
+    [x, NR0, NR1]]"
+
+function_compile_nat to_at_least_3_clause_single_def
+
+definition "to_at_least_3_clause_double i x y \<equiv>
+  [[x, y, Pos (RU (i, 0))], [x, y, Neg (RU (i, 0))]]"
+
+function_compile_nat to_at_least_3_clause_double_def
+
+lemma to_at_least_3_clause_eq: "to_at_least_3_clause xs i = (case xs of
+  [] => to_at_least_3_clause_empty1 i @ to_at_least_3_clause_empty2 i
+| [x] => to_at_least_3_clause_single i x
+| [x, y] => to_at_least_3_clause_double i x y
+| xs => [xs])"
+  unfolding to_at_least_3_clause_empty1_def to_at_least_3_clause_empty2_def Let_def
+    to_at_least_3_clause_single_def to_at_least_3_clause_double_def
+  by (induction xs i rule: to_at_least_3_clause.induct) simp_all
+
 function_compile_nat to_at_least_3_clause_eq
 
 fun at_most_three_sat_to_three_sat_aux_acc where
@@ -36,12 +102,22 @@ end
 context HOL_Nat_To_IMP_Minus
 begin
 
-lemmas to_at_least_3_clause_nat_eq = HTHN.to_at_least_3_clause_nat_eq_unfolded[unfolded
-  case_list_nat_def]
+compile_nat HTHN.to_at_least_3_clause_empty1_nat_eq_unfolded
+HOL_To_IMP_Minus_correct HOL_To_HOL_Nat.to_at_least_3_clause_empty1_nat by cook
+
+compile_nat HTHN.to_at_least_3_clause_empty2_nat_eq_unfolded
+HOL_To_IMP_Minus_correct HOL_To_HOL_Nat.to_at_least_3_clause_empty2_nat by cook
+
+compile_nat HTHN.to_at_least_3_clause_single_nat_eq_unfolded
+HOL_To_IMP_Minus_correct HOL_To_HOL_Nat.to_at_least_3_clause_single_nat by cook
+
+compile_nat HTHN.to_at_least_3_clause_double_nat_eq_unfolded
+HOL_To_IMP_Minus_correct HOL_To_HOL_Nat.to_at_least_3_clause_double_nat by cook
+
+lemmas to_at_least_3_clause_nat_eq = HTHN.to_at_least_3_clause_nat_eq_unfolded[
+  unfolded case_list_nat_def]
 compile_nat to_at_least_3_clause_nat_eq
-HOL_To_IMP_Minus_correct HOL_To_HOL_Nat.to_at_least_3_clause_nat
-  (* by cook *) \<comment>\<open>FIXME: too slow\<close>
-  sorry
+HOL_To_IMP_Minus_correct HOL_To_HOL_Nat.to_at_least_3_clause_nat by (cook mode = induction)
 
 lemmas at_most_three_sat_to_three_sat_aux_acc_nat_eq =
   HTHN.at_most_three_sat_to_three_sat_aux_acc_nat_eq_unfolded[unfolded case_list_nat_def]
