HOL_To_IMP-/HOL_Nat_To_IMP-/States/State_Update_Tracking.thy
@@ -17,13 +17,6 @@ lemma STATE_eq: "STATE s = s" unfolding STATE_def by simp
 text \<open>Prevent simplification of arguments\<close>
 lemma STATE_cong [cong]: "STATE s = STATE s" by simp
 
-lemma STATE_interp_state_State_eq: "STATE (interp_state (State s)) = s"
-  unfolding STATE_eq interp_state_def by simp
-
-lemma STATE_interp_update_retrieve_key_eq_if: "(STATE (interp_state (update_state s k v))) k' =
-  (if k = k' then v else (STATE (interp_state s)) k')"
-  unfolding STATE_eq SIMPS_TO_UNIF_eq SIMPS_TO_eq by simp
-
 lemma STATE_interp_retrieve_key_eqI:
   assumes "PROP SIMPS_TO_UNIF (STATE (interp_state st) k) val'"
   and "val' = val"
@@ -32,8 +25,19 @@ lemma STATE_interp_retrieve_key_eqI:
 
 lemma STATE_interp_update_eq_STATE_interp_fun_updI:
   assumes "PROP SIMPS_TO_UNIF val val'"
-  shows "STATE (interp_state (update_state st k val')) = (STATE (interp_state st))(k := val)"
-  using assms unfolding STATE_eq SIMPS_TO_UNIF_eq by simp
+  and "PROP SIMPS_TO_UNIF (update_state k val' st) s'"
+  shows "STATE (interp_state s') = (STATE (interp_state st))(k := val)"
+  using assms unfolding SIMPS_TO_UNIF_eq
+  by (simp flip: interp_update_state_eq add: STATE_eq)
+
+lemma STATE_interp_state_state_eq: "STATE (interp_state (state s)) = s"
+  unfolding STATE_eq interp_state_state_eq by simp
+
+lemma STATE_interp_update_retrieve_key_eq_if: "(STATE (interp_state (update_state k v s))) k' =
+  (if k = k' then v else (STATE (interp_state s)) k')"
+  unfolding STATE_eq SIMPS_TO_UNIF_eq SIMPS_TO_eq interp_update_state_eq by simp
+
+lemma string_eq_eq_True: "(s :: string) = s \<equiv> True" by simp
 
 ML_file\<open>state_update_tracking.ML\<close>
 
