HOL_To_IMP-/Refinements/HOL_To_IMP_Minus_SAT_To_AT_MOST_THREE_SAT.thy
@@ -1,3 +1,4 @@
+\<^marker>\<open>creator "Kevin Kappelmann"\<close>
 theory HOL_To_IMP_Minus_SAT_To_AT_MOST_THREE_SAT
   imports
     HOL_To_IMP_Minus_SAT
